theories/algos/unification.v
@@ -1,37 +1,32 @@
 From Coq Require Import String List Arith Lia.
-From minilog Require Import data utils.
+From minilog Require Import data utils substitutions.
 Import ListNotations.
 
 (** * Verified Unification Algorithm *)
 
 (** ** Finite substitutions and replacements *)
 
-Definition fin_subst := @fin_map pattern.
-
-Definition interp (f : fin_subst ) : psubstitution :=
-  fun x => match get f x with Some vx => vx | None => Pvar x end.
-
 Definition replace (p : pattern) (x : nat) (q : pattern) :=
-  psubst p (interp [(x, q)]).
+  psubst p (pinterp [(x, q)]).
 
-Notation "p '⟨' x ':=' q '⟩'" := (replace p x q) (at level 60).
-Notation "p '.⟨' s '⟩'" := (psubst p s) (at level 60).
+Notation "p '.[' x ':=' q ']'" := (replace p x q) (at level 60).
+Notation "p '.[' s ']'" := (psubst p s) (at level 60).
 
 (** Replacement in a list of equations of the forme [term = term] *)
 Definition replace_all_1 (l : list (pattern * pattern)) (x : nat) (p : pattern) :=
-  map (fun '(p1, p2) => (p1⟨x := p⟩, p2⟨x := p⟩)) l.
+  map (fun '(p1, p2) => (p1.[x := p], p2.[x := p])) l.
 
 (** Replacement in a list of equations of the form [var = term].
     Only the right hand sides are modified.
 *)
 Definition replace_all_2 (l : list (nat * pattern)) (x : nat) (p : pattern) :=
-  map (fun '(y, py) => (y, py⟨x := p⟩)) l.
+  map (fun '(y, py) => (y, py.[x := p])) l.
 
 (** ** Unifiers *)
 
 (** What it means that a substitution unifies 2 patterns *)
 Definition unifier u p1 p2 : Prop :=
-  p1.⟨u⟩ = p2.⟨u⟩.
+  p1.[u] = p2.[u].
 
 (** What it means to be a solution to a set of equations *)
 Definition satisfy (u : psubstitution) equs :=
@@ -39,8 +34,8 @@ Definition satisfy (u : psubstitution) equs :=
 
 Lemma unifier_cons:
   forall u f1 pat1 pats1 f2 pat2 pats2,
-    unifier u (Pcmp f1 (pat1::pats1)) (Pcmp f2 (pat2::pats2)) <->
-    (unifier u pat1 pat2 /\ unifier u (Pcmp f1 pats1) (Pcmp f2 pats2)).
+    unifier u (Papp f1 (pat1::pats1)) (Papp f2 (pat2::pats2)) <->
+    (unifier u pat1 pat2 /\ unifier u (Papp f1 pats1) (Papp f2 pats2)).
 Proof.
   intros. split.
   - intros H. inversion H; subst.
@@ -103,7 +98,7 @@ Definition unification_step (st : state) :=
   | [] => Success (solution st)
   | (t1, t2)::xs =>
     match t1, t2 with
-    | Pcmp f1 l1, Pcmp f2 l2 =>
+    | Papp f1 l1, Papp f2 l2 =>
       if (f1 =? f2)%string then
         match decompose l1 l2 with
         | Some equs => Update (Build_state (equs ++ xs) (solution st))
@@ -122,7 +117,7 @@ Lemma decompose_equiv:
   forall s1 s2 l1 l2 l,
     (s1 =? s2)%string = true ->
     decompose l1 l2 = Some l ->
-    equiv l [(Pcmp s1 l1, Pcmp s2 l2)].
+    equiv l [(Papp s1 l1, Papp s2 l2)].
 Proof.
   intros * ->%String.eqb_eq Hdec sub.
   induction l2 in l, l1, Hdec, sub |-*.
@@ -146,6 +141,109 @@ Proof.
       apply H2. now repeat econstructor.
 Qed.
 
+Lemma subst_replace_var:
+  forall x y sub pat,
+    sub x = sub y ->
+    pat.[sub] = pat.[x := Pvar y].[sub].
+Proof.
+  intros x y sub.
+  refine (pattern_induction _ _ _).
+  - intros z Heq1. unfold replace, pinterp. simpl.
+    destruct (x =? z)%nat eqn:Heq2; auto.
+    now apply Nat.eqb_eq in Heq2; subst.
+  - intros f dats Hdats Heq1. simpl. f_equal.
+    induction Hdats; auto.
+    specialize (H Heq1). simpl. now f_equal.
+Qed.
+
+Lemma subst_replace:
+  forall x px sub pat,
+    sub x = px.[sub] ->
+    pat.[sub] = pat.[x := px].[sub].
+Proof.
+  intros x px sub.
+  refine (pattern_induction _ _ _).
+  - intros y Heq1.
+    unfold replace, pinterp. simpl.
+    destruct (x =? y)%nat eqn:Heq2; auto.
+    now apply Nat.eqb_eq in Heq2; subst.
+  - intros f dats H1 H2.
+    simpl. f_equal.
+    rewrite map_map.
+    apply map_ext_in.
+    intros p Hp.
+    rewrite Forall_forall in H1.
+    now specialize (H1 _ Hp H2).
+Qed.
+
+Lemma replace_all_1_equiv':
+  forall equs sub x px,
+    sub x = px.[sub] ->
+    satisfy sub equs <->
+    satisfy sub (replace_all_1 equs x px).
+Proof.
+  intros.
+  induction equs as [| [pat1 pat2] equs IH]; try easy.
+  split; intros Hsat.
+  - inversion Hsat as [| ? ? H1 H2]; subst.
+    apply IH in H2.
+    econstructor; auto. red.
+    now do 2 rewrite <- subst_replace by auto.
+  - inversion Hsat as [| ? ? H1 H2]; subst.
+    apply IH in H2.
+    red in H1. do 2 rewrite <- subst_replace in H1 by auto.
+    now econstructor.
+Qed.
+
+Lemma replace_all_1_equiv:
+  forall equs sub x y,
+    sub x = sub y ->
+    satisfy sub equs <->
+    satisfy sub (replace_all_1 equs x (Pvar y)).
+Proof.
+  intros * H.
+  induction equs as [| [pat1 pat2] equs IH]; try easy.
+  split; intros Hsat.
+  + inversion Hsat as [| ? ? H1 H2]; subst.
+    apply IH in H2.
+    econstructor; auto. red.
+    now do 2 rewrite <- subst_replace_var by auto.
+  + inversion Hsat as [| ? ? H1 H2]; subst.
+    apply IH in H2.
+    red in H1. do 2 rewrite <- subst_replace_var in H1 by auto.
+    now econstructor.
+Qed.
+
+Lemma replace_all_2_equiv:
+  forall equs sub x y,
+    sub x = sub y ->
+    satisfy sub (map_as_equations equs) <->
+    satisfy sub (map_as_equations (replace_all_2 equs x (Pvar y))).
+Proof.
+  intros * H.
+  induction equs as [| [z patz] equs IH]; try easy.
+  split; intros Hsat.
+  + inversion Hsat as [| ? ? H1 H2]; subst.
+    apply IH in H2.
+    econstructor; auto. red.
+    now rewrite H1, <- subst_replace_var by auto.
+  + inversion Hsat as [| ? ? H1 H2]; subst.
+    apply IH in H2.
+    red in H1. rewrite <- subst_replace_var in H1 by auto.
+    now econstructor.
+Qed.
+
+Lemma unify_replace:
+  forall sub x patx pat1 pat2,
+    unifier sub (Pvar x) patx ->
+    unifier sub pat1 pat2 <->
+    unifier sub (pat1.[x := patx]) (pat2.[x := patx]).
+Proof.
+  intros. split; intros.
+  - red. now do 2 rewrite <- subst_replace by auto.
+  - red in H0. now do 2 rewrite <- subst_replace in H0 by auto.
+Qed.
+
 Theorem unification_step_equiv:
   forall st1 st2,
     unification_step st1 = Update st2 ->
@@ -158,11 +256,28 @@ Proof.
     inversion Hstep; subst. clear Hstep.
     apply Nat.eqb_neq in Heq1.
     unfold state_as_equations. simpl.
-    admit.
+    split.
+    + intros H. inversion H as [| ? ? H1 H2]; subst.
+      apply Forall_app in H2 as [H2 H3].
+      apply Forall_app. repeat econstructor; auto.
+      now apply replace_all_1_equiv.
+      now apply replace_all_2_equiv.
+    + intros [H1 H2]%Forall_app.
+      inversion H2 as [| ? ? H3 H4]; subst.
+      econstructor; auto.
+      apply replace_all_1_equiv in H1; auto.
+      apply replace_all_2_equiv in H4; auto.
+      now apply Forall_app; split.
   - destruct (existsb)%nat eqn:Heq1; try easy.
     inversion Hstep; subst. clear Hstep.
     unfold state_as_equations. simpl.
-    admit.
+    split.
+    + intros H. inversion H as [| ? ? H1 H2]; subst.
+      apply Forall_app in H2 as [H2 H3]. clear H.
+      apply Forall_app. repeat econstructor; auto.
+      now apply replace_all_1_equiv'.
+      admit.
+    + admit.
   - destruct (existsb)%nat eqn:Heq1; try easy.
     inversion Hstep; subst. clear Hstep.
     unfold state_as_equations. simpl.
