theories/data.v
@@ -8,27 +8,27 @@ Import ListNotations.
 
 (** A [datum] is function symbol applied to a set of [datum] *)
 Inductive datum :=
-  | Dcmp : string -> list datum -> datum.
+  | Dapp : string -> list datum -> datum.
 
-Definition Dcst (c : string) := Dcmp c [].
+Definition Dcst (c : string) := Dapp c [].
 
 (** Patterns over [datum] *)
 Inductive pattern :=
   | Pvar : nat -> pattern
-  | Pcmp : string -> list pattern -> pattern.
+  | Papp : string -> list pattern -> pattern.
 
-Definition Pcst (c : string) := Pcmp c [].
+Definition Pcst (c : string) := Papp c [].
 
 (** Free variables of a pattern *)
 Inductive free_var : pattern -> nat -> Prop :=
   | free_var_var x : free_var (Pvar x) x
-  | free_var_cmp x f l :
-    Exists (fun p => free_var p x) l -> free_var (Pcmp f l) x.
+  | free_var_app x f l :
+    Exists (fun p => free_var p x) l -> free_var (Papp f l) x.
 
 Fixpoint is_free (p : pattern) (x : nat) : bool :=
   match p with
   | Pvar y => (y =? x)%nat
-  | Pcmp _ pats => existsb (fun p => is_free p x) pats
+  | Papp _ pats => existsb (fun p => is_free p x) pats
   end.
 
 Axiom is_free_iff:
@@ -41,10 +41,10 @@ Axiom is_free_iff:
 *)
 Fixpoint datum_induction
   (P : datum -> Prop)
-  (Hind : forall f dats, Forall P dats -> P (Dcmp f dats))
+  (Hind : forall f dats, Forall P dats -> P (Dapp f dats))
   (dat : datum) : P dat :=
   match dat with
-  | Dcmp f dats =>
+  | Dapp f dats =>
     let helper := fix F l :=
       match l as l' return Forall P l' with
       | nil => Forall_nil P
@@ -61,11 +61,11 @@ Fixpoint datum_induction
 Fixpoint pattern_induction
   (P : pattern -> Prop)
   (H1 : forall x, P (Pvar x))
-  (Hind : forall f dats, Forall P dats -> P (Pcmp f dats))
+  (Hind : forall f dats, Forall P dats -> P (Papp f dats))
   (pat : pattern) : P pat :=
   match pat with
   | Pvar x => H1 x
-  | Pcmp f pats =>
+  | Papp f pats =>
     let helper := fix F l :=
       match l as l' return Forall P l' with
       | nil => Forall_nil P
@@ -83,21 +83,21 @@ Delimit Scope pattern with pattern.
 
 Fixpoint datum_size (d : datum) : nat :=
   match d with
-  | Dcmp _ dats =>
+  | Dapp _ dats =>
     1 + sum datum_size dats
   end.
 
 Fixpoint pattern_size (p : pattern) : nat :=
   match p with
   | Pvar _ => 1
-  | Pcmp _ pats =>
+  | Papp _ pats =>
     1 + sum pattern_size pats
   end.
 
 (** Boolean equality for [datum] *)
 Fixpoint datum_eqb (d1 d2 : datum) : bool :=
   match d1, d2 with
-  | Dcmp f1 l1, Dcmp f2 l2 =>
+  | Dapp f1 l1, Dapp f2 l2 =>
     let fix F l1 l2 :=
       match l1, l2 with
       | [], [] => true
@@ -132,7 +132,7 @@ Proof.
     apply Bool.andb_true_iff in H as [H1 H2].
     inversion_clear IH as [|? ? H3 H4].
     apply H3 in H1 as ->.
-    assert (Dcmp s dats = Dcmp s l).
+    assert (Dapp s dats = Dapp s l).
     apply IHl; auto.
     now inversion H.
   + destruct y; simpl in H; try easy.
@@ -149,65 +149,3 @@ Proof.
 Qed.
 
 Infix "=?" := (datum_eqb)%datum.
-
-(** ** First Order Substitution *)
-
-(** Closed substitutions (functions from variables to [datum]) *)
-Definition csubstitution := nat -> datum.
-
-(** Open substitutions (functions from variables to [pattern]) *)
-Definition psubstitution := nat -> pattern.
-
-(** Apply a closed substitution to a pattern *)
-Fixpoint csubst (p : pattern) (sub : csubstitution) : datum :=
-  match p with
-  | Pcmp f pats =>
-    Dcmp f (map (fun p => csubst p sub) pats)
-  | Pvar n => sub n
-  end.
-
-(** Apply an open substitution to a pattern *)
-Fixpoint psubst (p : pattern) (sub : psubstitution) : pattern :=
-  match p with
-  | Pcmp f pats =>
-    Pcmp f (map (fun p => psubst p sub) pats)
-  | Pvar n => sub n
-  end.
-
-(** What is means that a substitution is a matching for a [datum] and a [pattern] *)
-Definition Matching sub (dat : datum) (pat : pattern) : Prop :=
-  dat = csubst pat sub.
-
-(** What is means that a [pattern] matches a [datum] *)
-Definition Match (dat : datum) (pat : pattern) : Prop :=
-  exists sub, Matching sub dat pat.
-
-(** What is means that two patterns are unifiable *)
-Definition Unify (pat1 pat2 : pattern) : Prop :=
-  exists sub, psubst pat1 sub = psubst pat2 sub.
-
-(** Composing two subtitutions ([s2] after [s1]) *)
-Definition compose (s2 s1 : psubstitution) (n : nat) : pattern :=
-  psubst (s1 n) s2.
-
-Infix "•" := compose (at level 80).
-
-Definition equ (s1 s2 : psubstitution) :=
-  forall n, s1 n = s2 n.
-
-Infix "≡" := equ (at level 90).
-
-Definition subst_le (s1 s2 : psubstitution) : Prop :=
-  exists s3, s3 • s1 ≡ s2.
-
-Infix "⪯" := subst_le (at level 90).
-
-Lemma psubst_compose :
-  forall s1 s2 t, psubst t (s2 • s1) = psubst (psubst t s1) s2.
-Proof.
-  intros s1 s2. apply pattern_induction; simpl; try easy.
-  intros f ts Hts. induction ts; simpl; auto.
-  f_equal. inversion Hts; subst. rewrite H1.
-  specialize (IHts H2). clear H2.
-  simpl in IHts. now injection IHts as ->.
-Qed.
