theories/substitutions.v
@@ -1,0 +1,95 @@
+From Coq Require Import List String.
+From minilog Require Import utils data.
+Import ListNotations.
+
+(** * Substitutions and Unifiers *)
+
+(** Closed substitutions (functions from variables to [datum]) *)
+Definition csubstitution := nat -> datum.
+
+(** Open substitutions (functions from variables to [pattern]) *)
+Definition psubstitution := nat -> pattern.
+
+(** Apply a closed substitution to a pattern *)
+Fixpoint csubst (p : pattern) (sub : csubstitution) : datum :=
+  match p with
+  | Papp f pats =>
+    Dapp f (map (fun p => csubst p sub) pats)
+  | Pvar n => sub n
+  end.
+
+(** Apply an open substitution to a pattern *)
+Fixpoint psubst (p : pattern) (sub : psubstitution) : pattern :=
+  match p with
+  | Papp f pats =>
+    Papp f (map (fun p => psubst p sub) pats)
+  | Pvar n => sub n
+  end.
+
+Definition fin_csubst := (fin_map datum).
+Definition fin_psubst := (fin_map pattern).
+
+(** Intepreting a finite map as a csubstitution *)
+Definition cinterp (sub : fin_csubst) : csubstitution :=
+  fun x => match get sub x with None => Dcst "" | Some vx => vx end.
+
+(** Intepreting a finite map as a psubstitution *)
+Definition pinterp (sub : fin_psubst) : psubstitution :=
+  fun x => match get sub x with None => Pvar x | Some vx => vx end.
+
+Coercion cinterp : fin_csubst >-> csubstitution.
+Coercion pinterp : fin_psubst >-> psubstitution.
+
+(** ** Operations on substitutions *)
+
+Declare Scope subst.
+Delimit Scope subst with subst.
+
+(** Composing two subtitutions ([s2] after [s1]) *)
+Definition compose (s2 s1 : psubstitution) (n : nat) : pattern :=
+  psubst (s1 n) s2.
+
+Infix "•" := compose (at level 80) : subst.
+
+Definition equ (s1 s2 : psubstitution) :=
+  forall n, s1 n = s2 n.
+
+Infix "≡" := equ (at level 90) : subst.
+
+Definition subst_le (s1 s2 : psubstitution) : Prop :=
+  exists s3, (s3 • s1 ≡ s2)%subst.
+
+Infix "<=" := subst_le (at level 70).
+
+(** ** Matching *)
+
+(** What is means that a substitution is a matching for a [datum] and a [pattern] *)
+Definition Matching sub (dat : datum) (pat : pattern) : Prop :=
+  dat = csubst pat sub.
+
+(** What is means that a [pattern] matches a [datum] *)
+Definition Match (dat : datum) (pat : pattern) : Prop :=
+  exists sub, Matching sub dat pat.
+
+(** ** Unifiers *)
+
+(** What is means that to be a unifier *)
+Definition Unifier (sub : psubstitution) (pat1 pat2 : pattern) : Prop :=
+  psubst pat1 sub = psubst pat2 sub.
+
+Definition Mgu (sub : psubstitution) (pat1 pat2 : pattern) : Prop :=
+  Unifier sub pat1 pat2 /\ forall sub', Unifier sub' pat1 pat2 -> (sub <= sub')%subst.
+
+(** What is means that two patterns are unifiable *)
+Definition Unifiable (pat1 pat2 : pattern) : Prop :=
+  exists sub, Unifier sub pat1 pat2.
+
+Lemma psubst_compose :
+  forall s1 s2 t, psubst t (s2 • s1)%subst = psubst (psubst t s1) s2.
+Proof.
+  intros s1 s2. apply pattern_induction; simpl; try easy.
+  intros f ts Hts. induction ts; simpl; auto.
+  f_equal. inversion Hts; subst. rewrite H1.
+  specialize (IHts H2). clear H2.
+  simpl in IHts. now injection IHts as ->.
+Qed.
